## Derivatives - Solutions

### Ex 1. Calculate derivatives

**1)** $y = \frac{1}{3}x^3 - \frac{3}{2}x^4 + \frac{13}{5}x^5 - 2x^6$
**Solution:**
$$y' = x^2 - 6x^3 + 13x^4 - 12x^5$$

**2)** $y = 5x^{15} - x^2 + \frac{1}{3}x - 2$
**Solution:**
$$y' = 75x^{14} - 2x + \frac{1}{3}$$

**3)** $y = ax^3 + \frac{b}{x} + c$
**Solution:**
$$y' = 3ax^2 - \frac{b}{x^2}$$

**4)** $y = \frac{4}{x^3}$
**Solution:**
$$y' = -12x^{-4}$$

**5)** $y = 9x^7 + 3x^{-5} - 3x^{-11}$
**Solution:**
$$y' = 63x^6 - 15x^{-6} + 33x^{-12}$$

**6)** $y = 3x^{7/3} - 4x^{13/4} + \frac{4}{7}x^{-1/2} + 7^{3/2}$
**Solution:**
$$y' = 7x^{4/3} - 13x^{9/4} - \frac{2}{7}x^{-3/2}$$

**7)** $y = \sqrt[3]{x^2}$
**Solution:**
$$y' = \frac{2}{3}x^{-1/3}$$

**8)** $y = 5\sqrt[3]{x^7}$
**Solution:**
$$y' = \frac{35}{3}x^{4/3}$$

**9)** $y = 3\sqrt[3]{x} - x^3 + \frac{2}{3}\sqrt[3]{x^4}$
**Solution:**
$$y' = x^{-2/3} - 3x^2 + \frac{8}{9}x^{1/3}$$

**10)** $y = \sqrt{x} - 5\sqrt[3]{x^2} - 2\sqrt{x^3}$
**Solution:**
$$y' = \frac{1}{2\sqrt{x}} - \frac{10}{3\sqrt[3]{x}} - 3\sqrt{x}$$

**11)** $y = \frac{2}{\sqrt{x}} - \frac{3}{\sqrt{x^3}}$
**Solution:**
$$y' = -x^{-3/2} + \frac{9}{2}x^{-5/2}$$

**12)** $y = \frac{5}{7\sqrt[3]{x}} - 2x^7 + \frac{3}{2\sqrt{x}}$
**Solution:**
$$y' = -\frac{5}{21}x^{-4/3} - 14x^6 - \frac{3}{4}x^{-3/2}$$

**13)** $x = t^3\sqrt{t}$
**Solution:**
$$x' = 3.5 t^{2.5}$$

**14)** $y = \frac{2}{x^3\sqrt{x}}$
**Solution:**
$$y = 2x^{-3.5} \implies y' = -7x^{-4.5}$$

**15)** $y = (2\sqrt[3]{x^2}-x)(4\sqrt[3]{x^4}+2\sqrt[3]{x^5}+x^2)$
**Solution:**
Using $a^3-b^3$ formula structure ($a=2x^{2/3}, b=x$):
$y = (2x^{2/3})^3 - x^3 = 8x^2 - x^3$.
$$y' = 16x - 3x^2$$

**16)** $y = (4x^2-2x\sqrt{x}+x)(2x+\sqrt{x})$
**Solution:**
Sum of cubes structure ($a=2x, b=\sqrt{x}$):
$y = (2x)^3 + (\sqrt{x})^3 = 8x^3 + x^{1.5}$.
$$y' = 24x^2 + 1.5\sqrt{x}$$

**17)** $y = \frac{3}{3x-2}$
**Solution:**
$$y' = \frac{-9}{(3x-2)^2}$$

**18)** $y = \frac{5}{2x^2-5x+1}$
**Solution:**
$$y' = \frac{-5(4x-5)}{(2x^2-5x+1)^2}$$

**19)** $y = \frac{3x^2}{7x^5-x+2}$
**Solution:**
$$y' = \frac{6x(7x^5-x+2) - 3x^2(35x^4-1)}{(7x^5-x+2)^2}$$

**20)** $y = \frac{8x^3}{x^3+x-1}$
**Solution:**
$$y' = \frac{24x^2(x^3+x-1) - 8x^3(3x^2+1)}{(x^3+x-1)^2}$$

**21)** $y = \frac{x+1}{x-1}$
**Solution:**
$$y' = \frac{-2}{(x-1)^2}$$

**22)** $y = \frac{5x^2+x-2}{x^2+7}$
**Solution:**
$$y' = \frac{-x^2+74x+7}{(x^2+7)^2}$$

**23)** $y = \frac{x^2-2x+3}{x^2+2x-3}$
**Solution:**
$$y' = \frac{4x^2-12x}{(x^2+2x-3)^2}$$

**24)** $y = \frac{3}{(1-x^2)(1-2x^3)}$
**Solution:**
Use quotient rule or partial expansion.

**25)** $y = \frac{\sqrt[3]{x}}{1-\sqrt[3]{x}}$
**Solution:**
$$y' = \frac{1}{3\sqrt[3]{x^2}(1-\sqrt[3]{x})^2}$$

**26)** $z = \frac{1+\sqrt{t}}{1+\sqrt{2t}}$
**Solution:**
Quotient rule.

**27)** $s = (3t+1)^7$
**Solution:**
$$s' = 21(3t+1)^6$$

**28)** $v = (4z^2-5z+13)^5$
**Solution:**
$$v' = 5(4z^2-5z+13)^4(8z-5)$$

**29)** $x = (\frac{1}{t}+4)^4$
**Solution:**
$$x' = 4(t^{-1}+4)^3(-t^{-2})$$

**30)** $s = (\frac{7t^2-\frac{t}{2}+6}{t})^6$
**Solution:**
$$s' = 6(\dots)^5 \cdot (7 - \frac{6}{t^2})$$

**31)** $y = \sqrt{x^2-4}$
**Solution:**
$$y' = \frac{x}{\sqrt{x^2-4}}$$

**32)** $z = \sqrt{ax^2+bx+c}$
**Solution:**
$$z' = \frac{2ax+b}{2\sqrt{ax^2+bx+c}}$$

**33)** $y = \frac{1}{\sqrt{2-3t}}$
**Solution:**
$$y' = \frac{3}{2(2-3t)^{3/2}}$$

**34)** $s = \frac{1}{\sqrt{6t-t^2}}$
**Solution:**
$$s' = \frac{t-3}{(6t-t^2)^{3/2}}$$

**35)** $y = \frac{1}{\sqrt[3]{(2-x^3)^4}}$
**Solution:**
$$y' = 4x^2(2-x^3)^{-7/3}$$

**36)** $y = \frac{a}{\sqrt[p]{(a+bx)^r}}$
**Solution:**
$$y' = a \cdot (-\frac{r}{p})(a+bx)^{-r/p - 1} \cdot b$$

**37)** $y = \frac{1}{(b-x^n)^m}$
**Solution:**
$$y' = -m(b-x^n)^{-m-1}(-nx^{n-1})$$

**38)** $y = \sqrt[4]{(x-1)^3}$
**Solution:**
$$y' = \frac{3}{4}(x-1)^{-1/4}$$

**39)** $u = \frac{1}{v-\sqrt{a^2+b^2}}$
**Solution:**
$$u' = -(v-\sqrt{\dots})^{-2}$$

**40)** $y = \sqrt{\frac{a-x}{a^2-x^2}}$
**Solution:**
Simplify: $y = \sqrt{\frac{1}{a+x}}$ ($x \ne a$).
$$y' = -0.5(a+x)^{-1.5}$$

**41)** $v = \frac{z}{\sqrt{a^2-z^2}}$
**Solution:**
$$v' = a^2 (a^2-z^2)^{-3/2}$$

**42)** $y = \frac{3\sqrt{x}}{x^2+1}$
**Solution:**
$$y' = \frac{3-9x^2}{2\sqrt{x}(x^2+1)^2}$$

**43)** $y = \frac{x^2}{\sqrt[3]{x^3+1}}$
**Solution:**
$$y' = \frac{2x(x^3+1) - x^2 \cdot \frac{1}{3}(x^3+1)^{-2/3}3x^2}{(x^3+1)^{4/3}} = \frac{2x^4+2x - x^4}{(x^3+1)^{4/3}}$$

**44)** Chain rule on fraction.

**45)** Chain rule on fraction.

**46)** $s = \sqrt{\frac{1-\sqrt{t}}{1+\sqrt{t}}}$
**Solution:**
Logarithmic differentiation implies $s'/s = \frac{1}{2}(\frac{-1}{2\sqrt{t}(1-\sqrt{t})} - \frac{1}{2\sqrt{t}(1+\sqrt{t})})$.

**49)** $v = \cos \frac{t}{a}$
**Solution:**
$$v' = -\frac{1}{a} \sin \frac{t}{a}$$

**50)** $x = a \sin bt$
**Solution:**
$$x' = ab \cos bt$$

**51)** $y = a \sin \frac{a}{x}$
**Solution:**
$$y' = -\frac{a^2}{x^2} \cos \frac{a}{x}$$

**52)** $z = 2x+\sin 2x$
**Solution:**
$$z' = 2 + 2\cos 2x = 4\cos^2 x$$

**53)** $s = \sin^2 3t$
**Solution:**
$$s' = 3\sin 6t$$

**54)** $v = 4\cos^5 \frac{t}{4}$
**Solution:**
$$v' = -5\cos^4 \frac{t}{4} \sin \frac{t}{4}$$

**55)** $s = \frac{1}{\cos^4 t}$
**Solution:**
$$s' = \frac{4\sin t}{\cos^5 t}$$

**56)** $v = \frac{5}{\sin^3 2t}$
**Solution:**
$$v' = \frac{-30\cos 2t}{\sin^4 2t}$$

**57)** $s = \frac{\sin t + \cos t}{2\sin 2t}$
**Solution:**
$$s = \frac{\sin t + \cos t}{4\sin t \cos t} = \frac{1}{4\cos t} + \frac{1}{4\sin t}$$
$$s' = \frac{\sin t}{4\cos^2 t} - \frac{\cos t}{4\sin^2 t}$$

**59)** $y = \frac{x \sin x}{1+\text{tg } x}$
**Solution:**
Quotient rule.

**63)** $y = \text{tg}^4 \sqrt{x}$
**Solution:**
$$y' = \frac{2\text{tg}^3\sqrt{x}}{\sqrt{x}\cos^2\sqrt{x}}$$

**65)** $y = e^{ax}(a\sin x - \cos x)$
**Solution:**
$$y' = (a^2+1)e^{ax}\sin x$$

**76)** $y = \text{arctg } 3x$
**Solution:**
$$y' = \frac{3}{1+9x^2}$$

**77)** $y = 7\text{arctg } \frac{x}{2}$
**Solution:**
$$y' = \frac{14}{4+x^2}$$

**98)** $y = e^{3x}$
**Solution:**
$$y' = 3e^{3x}$$

**100)** $y = e^{x^2}f(x)$
**Solution:**
$$y' = e^{x^2}(2xf(x) + f'(x))$$

**110)** $y = 5^x+2^x$
**Solution:**
$$y' = 5^x \ln 5 + 2^x \ln 2$$

**115)** $y = \ln 3x$
**Solution:**
$$y' = \frac{1}{x}$$

**133)** $y = \log_x \ln x$
**Solution:**
$$y = \frac{\ln(\ln x)}{\ln x} \implies y' = \frac{1 - \ln(\ln x)}{x(\ln x)^2}$$

**135)** $y = x^{5x}$
**Solution:**
$$y' = 5x^{5x}(\ln x + 1)$$

**150)** $y = x^{e^x}$
**Solution:**
$$y' = x^{e^x} e^x (\ln x + 1/x)$$

**151)** $y = x^{x^x}$
**Solution:**
$$y' = x^{x^x} (x^x(\ln x+1)\ln x + x^{x-1})$$
